\documentclass{article}
\usepackage{epsfig}
% Packages requested by user
\usepackage{amsmath}
\usepackage{amsfonts}
\usepackage{amssymb}
\usepackage{amsthm}

\pagestyle{empty}
\begin{document}
\begin{eqnarray} \frac{du}{dt} & = & \frac{-u}{STP\_tau\_u} + STP\_U (1-u^-) \delta(t-t_{spk}) \\ \frac{dx}{dt} & = & \frac{1-x}{STP\_tau\_x} - u^+ x^- \delta(t-t_{spk}) \\ \frac{dI}{dt} & = & \frac{-I}{\tau_S} + A u^+ x- \delta(t-t_{spk}) \end{eqnarray}
\pagebreak

\[ STDP(t) = \begin{cases} \alpha^+(1-(1-e^{-\frac{t}{\tau^+}})(\frac{1+e^{-\frac{\gamma}{\tau^+}}}{1-e^{-\frac{\gamma}{\tau^+}}})) & \text{if } t < \gamma \\ -\alpha^+ e^{-\frac{t}{\tau^+}} & \text{if } t \geq \gamma \end{cases} \]
\pagebreak

\begin{align*} \frac{dv}{dt} = & ~ 0.04v^2 + 5v + 140 - u + I & \text{(1)}\\ \frac{du}{dt} = & ~ a (bv - u) & \text{(2)} \end{align*}
\pagebreak

$v$
\pagebreak

$I$
\pagebreak

$I = i_{syn} + I_{ext}$
\pagebreak

$u$
\pagebreak

$a$
\pagebreak

$b$
\pagebreak

$t$
\pagebreak

$a, b, c, d$
\pagebreak

$v_{cutoff}=+30$
\pagebreak

\begin{align*} v(v>30) = & ~ c & \text{(3)}\\ u(v>30) = & ~ u + d & \text{(4)}\end{align*}
\pagebreak

$a=0.02, b=0.2, c=-65, d=8$
\pagebreak

$a=0.1, b=0.2, c=-65, d=2)$
\pagebreak

\begin{align*} \frac{dv}{dt} = & ~ (k (v - vr) (v - vt) - u + I) / C & \text{(5)}\\ \end{align*}
\pagebreak

$k$
\pagebreak

$vr$
\pagebreak

$vt$
\pagebreak

$C$
\pagebreak

\begin{align*} \frac{dv}{dt} = & ~ a (b (v - vr) - u) & \text{(6)}\\ \end{align*}
\pagebreak

$C, k, vr, vt, a, b, vpeak, c, d$
\pagebreak

$v_{cutoff}=+vpeak$
\pagebreak

\begin{align*} v(v>vpeak) = & ~ c & \text{(7)}\\ u(v>vpeak) = & ~ u + d & \text{(8)}\end{align*}
\pagebreak

$C=100, k=0.7, vr=-60, vt=-40, a=0.03, b=-2.0, vpeak=35, c=-50, d=100$
\pagebreak

$C=20, k=1, vr=-55, vt=-40, a=0.15, b=8, vpeak=25, c=-55, d=200)$
\pagebreak

$i_{dendr}$
\pagebreak

$I = i_{syn} + i_{dendr} + I_{ext}$
\pagebreak

\begin{align*} i_{dendr} = & G_{down} (v - v_{down}) + \sum \limits_{up} G_{up} (v - v_{up}) & \text{(9)} \end{align*}
\pagebreak

$G_{up}$
\pagebreak

$G_{down}$
\pagebreak

$j$
\pagebreak

$ I_{j}^{syn} $
\pagebreak

$i$
\pagebreak

\begin{align*} I_{j}^{syn} = & ~ \sum \limits_{i=1}^{N} s_{ij}w_{ij} & \text{(5)} \end{align*}
\pagebreak

$s_{ij}$
\pagebreak

$w_{ij}$
\pagebreak

$I_{ij}$
\pagebreak

\begin{align*} I_{j}^{syn} = & ~ \sum \limits_{i=1}^{N} i_{ij}w_{ij} & \text{(6)} \end{align*}
\pagebreak

$i,j$
\pagebreak

$g$
\pagebreak

$i_{e}$
\pagebreak

$i_{i}$
\pagebreak

\begin{align*} i_{e} = & ~ i_{NMDA} + i_{AMPA} & \text{(7)} \\ i_{i} = & ~ i_{GABA_{A}} + i_{GABA_{B}} & \text{(8)} \end{align*}
\pagebreak

$i_{AMPA}$
\pagebreak

$i_{NMDA}$
\pagebreak

\begin{align*} i_{AMPA} = & ~ g_{AMPA}(v-v^{rev}_{AMPA}) & \text{(9)} \\ i_{NMDA} = & ~ g_{NMDA}\frac{\Big[\frac{v+80}{60} \Big]^{2}}{1+\Big[\frac{v+80}{60} \Big]^{2}} (v-v^{rev}_{NMDA}) & \text{(10)} \end{align*}
\pagebreak

$v^{rev}$
\pagebreak

$i_{GABA_A}$
\pagebreak

$i_{GABA_B}$
\pagebreak

\begin{align*} i_{GABA_{A}} = & ~ g_{GABA_{A}}(v-v^{rev}_{GABA_{A}}) & \text{(11)} \\ i_{GABA_{B}} = & ~ g_{GABA_{B}}(v-v^{rev}_{GABA_{B}}) & \text{(12)} \end{align*}
\pagebreak

\begin{align*} g_{k} = & ~ \sum \limits_{f} e^{t-t_{f}/ \tau} \Theta(t-t_f) & \text{(13)} \end{align*}
\pagebreak

$f$
\pagebreak

$t_f$
\pagebreak

$ \Theta $
\pagebreak

$\sigma$
\pagebreak

$ (pre.x-post.x)^2/a^2 + (pre.y-post.y)/b^2 <= 1 $
\pagebreak

$pre.z==post.z$
\pagebreak

$ (pre.x-post.x)^2/a^2 + (pre.y-post.y)/b^2 == 1$
\pagebreak

$ pre.x = pre.x / gridPre.x * gridPost.x $
\pagebreak

$ pre.y = pre.y / gridPre.y * gridPost.y $
\pagebreak

$ pre.z = pre.z / gridPre.z * gridPost.z $
\pagebreak

$i_{10}$
\pagebreak

\begin{align*} i_{10} = & G_0^{down} (v_{10} - v_{0}) + G_5^{down} (v_{10} - v_{5}) + G_{15}^{up} (v_{10} - v_{15}), & \text{(1)} \end{align*}
\pagebreak

$v_n$
\pagebreak

$G_n^{down}$
\pagebreak

$G_n^{up}$
\pagebreak

$ \Delta t = t_{post} - t_{pre} $
\pagebreak

$ \Delta t $
\pagebreak

$ \Delta t < 0 $
\pagebreak

$ \Delta t>0 $
\pagebreak

$ \Delta \vert w \vert $
\pagebreak

$ \Delta t > 0 $
\pagebreak

$ \Delta w = A_{+} \exp(-\Delta t/\tau_{+}) $
\pagebreak

$ \Delta t <= 0 $
\pagebreak

$ \Delta w = A_{-} \exp(-\Delta t/\tau_{-}) $
\pagebreak

$ A_{+}$
\pagebreak

$ A_{-}$
\pagebreak

$ \tau_{+} $
\pagebreak

$\tau_{-}$
\pagebreak

\[ \frac{dw_{i,j}}{dt} = \delta + \beta(\mbox{pre-before-post}_{i,j} + \mbox{pre-after-post}_{i,j}) \]
\pagebreak

$ w_{i,j} $
\pagebreak

$ \delta $
\pagebreak

$ \beta $
\pagebreak

$ \mbox{pre-before-post}_{i,j} $
\pagebreak

$ \mbox{pre-after-post}_{i,j} $
\pagebreak

\[ \frac{dw_{i,j}}{dt} = \bigg[ \alpha \cdot w_{i,j} \Big(1-\frac{R_{avg}}{R_{target}} \Big) + \beta \cdot (\mbox{pre-before-post}_{i,j} + \mbox{pre-after-post}_{i,j}) \bigg] \cdot K \]
\pagebreak

$ \frac{dw_{i,j}}{dt} $
\pagebreak

$ K $
\pagebreak

$ \alpha $
\pagebreak

$ R_{avg} $
\pagebreak

$ R_{target} $
\pagebreak

\[ K=\frac{R_{avg}}{T \cdot \Big( 1 + \vert 1- R_{avg}/R_{target} \vert \cdot \gamma \Big) } \]
\pagebreak

$ T $
\pagebreak

$ \gamma $
\pagebreak

$ \alpha = 0.1 $
\pagebreak

$ T = 10.0 $
\pagebreak

\end{document}
